feat: Encodable Term

Logic/Predicate/Coding.lean
@@ -1,53 +1,53 @@
 import Logic.Predicate.Term
 import Mathlib.Data.W.Basic
 
-variable {L : Language} [∀ k, Encodable (L.func k)] {μ : Type _} [Encodable μ]
+variable {L : Language} [∀ k, Encodable (L.func k)] {μ : Type _} [Inhabited μ] [Encodable μ]
 
 namespace SubTerm
 open Encodable
-variable (L) (μ) (n : ℕ)
+variable {n : ℕ}
 
-private def Label := Fin n ⊕ μ ⊕ Σ n, L.func n
+-- 本来 " + 1"は必要ないがofNatの停止性の証明がより簡易になるためつけている
+def toNat : SubTerm L μ n → ℕ 
+  | #x                    => (Nat.bit false $ Nat.bit false (encode x)) + 1
+  | &x                    => (Nat.bit false $ Nat.bit true (encode x)) + 1
+  | func (arity := k) f v => (Nat.bit true  $ Nat.mkpair k $
+      Nat.mkpair (encode f) (Fin.finitaryToNat $ fun i => (v i).toNat)) + 1
 
-@[reducible]
-def LabelType : Label L μ n → Type
-  | Sum.inl _                => Empty
-  | Sum.inr $ Sum.inl _      => Empty
-  | Sum.inr $ Sum.inr ⟨k, _⟩ => Fin k
+#eval toNat (&9 : SyntacticSubTerm Language.equal 0)
 
-variable {L μ n}
+def ofNat : ℕ → Option (SubTerm L μ n)
+| 0  => none
+| e + 1 =>
+  match e.bodd with
+  | false => 
+    match e.div2.bodd with
+    | false => (decode₂ (Fin n) e.div2.div2).map fixedVar
+    | true  => (decode₂ μ e.div2.div2).map freeVar
+  | true  =>
+      let x := e.div2
+      let k := x.unpair.1
+      let f' : Option (L.func k) := decode₂ (L.func k) x.unpair.2.unpair.1
+      let w : Fin k → ℕ := Nat.unvector x.unpair.2.unpair.2
+      have : ∀ i, w i < e + 1 := fun i =>
+        Nat.lt_succ_of_le (le_trans (Nat.unvector_le x.unpair.2.unpair.2 i)
+          (le_trans (Nat.unpair_right_le _) $
+            le_trans (Nat.unpair_right_le _) $ by simpa[Nat.div2_val] using Nat.div_le_self e 2))
+      let v' : Option (Fin k → SubTerm L μ n) := Fin.toOptionFinTo (fun i => ofNat (w i))
+      func <$> f' <*> v'
+  decreasing_by exact this i
 
-@[reducible] def ofW : WType (LabelType L μ n) → SubTerm L μ n
-  | ⟨Sum.inl x,                _⟩ => #x
-  | ⟨Sum.inr $ Sum.inl x,      _⟩ => &x
-  | ⟨Sum.inr $ Sum.inr ⟨_, f⟩, F⟩ => func f (fun x => ofW (F x))
+@[simp] lemma ofNat_toNat : ∀ t : SubTerm L μ n, ofNat (toNat t) = some t
+  | #x => by simp[ofNat, toNat]; rw[Nat.bodd_bit, Nat.div2_bit]; simp; rw[Nat.bodd_bit, Nat.div2_bit]; simp
+  | &x => by simp[ofNat, toNat]; rw[Nat.bodd_bit, Nat.div2_bit]; simp; rw[Nat.bodd_bit, Nat.div2_bit]; simp
+  | func f v => by
+      simp[ofNat, toNat]
+      rw[Nat.bodd_bit, Nat.div2_bit, Nat.unpair_mkpair]; simp[fun i => ofNat_toNat (v i)];
 
-def toW : SubTerm L μ n → WType (LabelType L μ n)
-  | #x         => ⟨Sum.inl x, Empty.rec⟩
-  | &x         => ⟨Sum.inr $ Sum.inl x, Empty.rec⟩
-  | (func f v) => ⟨Sum.inr $ Sum.inr ⟨_, f⟩, fun i => toW (v i)⟩
-
-def equivW : SubTerm L μ n ≃ WType (LabelType L μ n) where
-  toFun     := toW
-  invFun    := ofW
-  left_inv  := by intros t; induction t <;> simp[*, toW]
-  right_inv := by
-    intros w; induction' w with l F ih
-    rcases l with (n | b | ⟨k, f⟩) <;> simp[*, ofW, toW]
-
-instance : ∀ t, Fintype (LabelType L μ n t)
-  | Sum.inl _                => Fintype.ofIsEmpty
-  | Sum.inr $ Sum.inl _      => Fintype.ofIsEmpty
-  | Sum.inr $ Sum.inr ⟨k, _⟩ => Fin.fintype k
-
-instance : ∀ t, Encodable (LabelType L μ n t)
-  | Sum.inl _                => IsEmpty.toEncodable
-  | Sum.inr $ Sum.inl _      => IsEmpty.toEncodable
-  | Sum.inr $ Sum.inr ⟨k, _⟩ => Fin.encodable k
-
-instance : Encodable (Label L μ n) := Sum.encodable
-
-instance : Encodable (SubTerm L μ n) := Encodable.ofEquiv _ equivW
+instance : Encodable (SubTerm L μ n) where
+  encode := toNat
+  decode := ofNat
+  encodek := ofNat_toNat
 
 end SubTerm
 
